Fix ec specs to match final yul model (#27)

src/specs/PointAddIntoDest.ec
@@ -6,52 +6,41 @@ require import Logic.
 require import Memory.
 require import PurePrimops.
 require import Real.
+require import RevertWithMessage.
 require import UInt256.
 require import Utils.
 require import YulPrimops.
 require import Verifier.
 
-import MemoryMap.
-
 module PointAddIntoDest = {
-  proc low(usr_p1, usr_p2, usr_dest) =
+  proc low(p1, p2, dest) =
   {
-    var _1, _5, _6, _9, _13, _14, tmp64;
-    _1 <@ Primops.mload(usr_p1);
+    var _1, _5, _6, _9, _13, _14;
+    _1 <@ Primops.mload(p1);
     Primops.mstore(W256.of_int 0, _1);
-    _5 <@ Primops.mload(usr_p1 + W256.of_int 32);
+    _5 <@ Primops.mload(p1 + W256.of_int 32);
     Primops.mstore(W256.of_int 32, _5);
-    _6 <@ Primops.mload(usr_p2);
+    _6 <@ Primops.mload(p2);
     Primops.mstore(W256.of_int 64, _6);
-    _9 <@ Primops.mload(usr_p2 + W256.of_int 32);
+    _9 <@ Primops.mload(p2 + W256.of_int 32);
     Primops.mstore(W256.of_int 96, _9);
     _13 <@ Primops.gas();
-    _14 <@ Primops.staticcall(_13, W256.of_int 6, W256.zero, W256.of_int 128, usr_dest, W256.of_int 64);
+    _14 <@ Primops.staticcall(_13, W256.of_int 6, W256.zero, W256.of_int 128, dest, W256.of_int 64);
     if ((bool_of_uint256 (PurePrimops.iszero _14)))
-      {
-      tmp64 <@ Verifier.usr_revertWithMessage((W256.of_int 30), (W256.of_int STRING (*pointAddIntoDest: ecAdd failed*)));
-      }
+    {
+      RevertWithMessage.low((W256.of_int 30), (W256.of_int STRING (*pointAddIntoDest: ecAdd failed*)));
+    }
   }
 }.
 
-lemma usr_pointAddIntoDest_actual_matches_low (x y : uint256) : equiv [
-    Verifier.usr_pointAddIntoDest ~ PointAddIntoDest.low :
-      ={Primops.memory} /\
-      ={arg} /\
-      ={Primops.reverted} /\
-      !Primops.reverted{1}
-      ==>
-        (Primops.reverted{1} <=> Primops.reverted{2}) /\
-        (!Primops.reverted{1}) =>
-        forall (idx: uint256),
-        Primops.memory{1}.[idx] =
-        Primops.memory{2}.[idx]
+lemma usr_pointAddIntoDest_extracted_matches_low (x y : uint256) : equiv [
+    Verifier_1261.usr_pointAddIntoDest ~ PointAddIntoDest.low :
+      ={arg, glob PointAddIntoDest} ==>
+      ={res, glob PointAddIntoDest}
     ].
 proof.
   proc.
-  seq 24 10: (#pre /\ ={_1, _5, _6, _9, _13, _14} /\ _2{1} = W256.zero /\ _3{1} = W256.of_int 32 /\ _4{1} = usr_p1{1} + _3{1}
-             /\ _7{1} = W256.of_int 64 /\ _8{1} = usr_p2{1} + _3{1} /\ _10{1} = W256.of_int 96 /\ _11{1} = W256.of_int 128
-             /\ _12{1} = W256.of_int 6).
-  inline*. wp. skip. progress.
-  inline*. wp. skip. progress.
+  seq 24 10: (#pre /\ ={_14}).
+  inline*. wp. skip. by progress.
+  inline*. wp. skip. by progress.
 qed.
