src/specs/PointSubAssign.ec
@@ -1,58 +1,48 @@
 pragma Goals:printall.
 
 require import Array.
+require        Constants.
 require import EllipticCurve.
 require import Logic.
 require import Memory.
 require import PurePrimops.
 require import Real.
+require import RevertWithMessage.
 require import UInt256.
 require import Utils.
 require import YulPrimops.
 require import Verifier.
 
-import MemoryMap.
-
 module PointSubAssign = {
-  proc low(usr_p1, usr_p2) =
+  proc low(p1, p2) =
   {
-    var _1, _5, _6, _9, _15, _16, tmp71;
-    _1 <@ Primops.mload(usr_p1);
+    var _1, _5, _6, _9, _15, _16;
+    _1 <@ Primops.mload(p1);
     Primops.mstore(W256.zero, _1);
-    _5 <@ Primops.mload(usr_p1 + W256.of_int 32);
+    _5 <@ Primops.mload(p1 + W256.of_int 32);
     Primops.mstore(W256.of_int 32, _5);
-    _6 <@ Primops.mload(usr_p2);
+    _6 <@ Primops.mload(p2);
     Primops.mstore(W256.of_int 64, _6);
-    _9  <@ Primops.mload(usr_p2 + W256.of_int 32);
-    Primops.mstore(W256.of_int 96, W256.of_int 21888242871839275222246405745257275088696311157297823662689037894645226208583 - _9);
+    _9  <@ Primops.mload(p2 + W256.of_int 32);
+    Primops.mstore(W256.of_int 96, W256.of_int Constants.Q - _9);
     _15 <@ Primops.gas();
-    _16 <@ Primops.staticcall(_15, W256.of_int 6, W256.zero, W256.of_int 128, usr_p1, W256.of_int 64);
+    _16 <@ Primops.staticcall(_15, W256.of_int 6, W256.zero, W256.of_int 128, p1, W256.of_int 64);
     if ((bool_of_uint256 (PurePrimops.iszero _16)))
-      {
-      tmp71 <@ Verifier.usr_revertWithMessage(W256.of_int 28, (W256.of_int STRING));
-      }
+    {
+      RevertWithMessage.low(W256.of_int 28, (W256.of_int STRING));
+    }
   }
 }.
 
-lemma usr_pointSubAssign_actual_matches_low (x y : uint256) : equiv [
-    Verifier.usr_pointSubAssign ~ PointSubAssign.low :
-      ={Primops.memory} /\
-      ={arg} /\
-      ={Primops.reverted} /\
-      !Primops.reverted{1}
-      ==>
-        (Primops.reverted{1} <=> Primops.reverted{2}) /\
-        (!Primops.reverted{1}) =>
-        forall (idx: uint256),
-        Primops.memory{1}.[idx] =
-        Primops.memory{2}.[idx]
-      ].
+lemma usr_pointSubAssign_extracted_matches_low :
+    equiv [
+      Verifier_1261.usr_pointSubAssign ~ PointSubAssign.low :
+      ={arg, glob PointSubAssign} ==>
+      ={res, glob PointSubAssign}
+    ].
 proof.
   proc.
-  seq 16 7: (#pre /\ ={_1} /\ _2{1} = W256.zero /\ _3{1} = W256.of_int 32 /\ _4{1} = usr_p1{1} + _3{1}
-            /\ ={_5, _6, _9} /\ _7{1} = W256.of_int 64 /\ _8{1} = usr_p2{1} + _3{1}).
-  inline*. wp. skip. progress. sp.
-  seq 7 3: (#pre /\ _13{1} = W256.of_int 128 /\ _14{1} = W256.of_int 6 /\ ={_15, _16}).
-  inline*. wp. skip. progress.
-  inline*. wp. skip. progress.
+  seq 26 10: (#pre /\ ={_16}).
+  inline*. wp. skip. rewrite /Constants.Q. by progress.
+  inline*. wp. skip. by progress.
 qed.  
